Make serialization and deserialization verify
Include AAD Length in AAD Validity.
Corrected definition of AAD Length to include the two bytes that record the number of key/value pairs.
State and prove some needed lemmas.

src/SDK/MessageHeader/SerializeAAD.dfy
@@ -12,43 +12,92 @@ module MessageHeader.SerializeAAD {
   import opened StandardLibrary
   import opened UInt = StandardLibrary.UInt
 
-  lemma {:axiom} Assume(b: bool)
-    ensures b
-
-  function EncCtxToSeqRec(kvPairs: EncCtx, i: nat): seq<uint8>
-    requires forall i :: 0 <= i < |kvPairs| ==> |kvPairs[i].0| < UINT16_LIMIT && |kvPairs[i].1| < UINT16_LIMIT
-    decreases |kvPairs| - i
-  {
-    if i < |kvPairs| then
-      UInt16ToSeq(|kvPairs[i].0| as uint16) + kvPairs[i].0[..] +
-      UInt16ToSeq(|kvPairs[i].1| as uint16) + kvPairs[i].1[..] +
-      EncCtxToSeqRec(kvPairs, i + 1)
-    else
-      []
-  }
-
-  function EncCtxToSeq(kvPairs: EncCtx): (ret: seq<uint8>)
-    requires forall i :: 0 <= i < |kvPairs| ==> |kvPairs[i].0| < UINT16_LIMIT && |kvPairs[i].1| < UINT16_LIMIT
-    ensures |ret| < UINT16_LIMIT // TODO: we need to establish that this length fits into two bytes
-  {
-    Assume(|EncCtxToSeqRec(kvPairs, 0)| < UINT16_LIMIT);  // TODO
-    EncCtxToSeqRec(kvPairs, 0)
-  }
+  // ----- Specification -----
 
   function SerializeAAD(aad: T_AAD): seq<uint8>
     requires ValidAAD(aad)
   {
-    match aad {
-      case AAD(kvPairs) =>
-        Assume(forall i :: 0 <= i < |kvPairs| ==> |kvPairs[i].0| < UINT16_LIMIT && |kvPairs[i].1| < UINT16_LIMIT);
-        var encCtxSeq := EncCtxToSeq(kvPairs);
-        UInt16ToSeq(|encCtxSeq| as uint16) +
-        // It would be nicer if this could be a flatten + map as for AAD
-        UInt16ToSeq(Assume(|kvPairs| < UINT16_LIMIT); |kvPairs| as uint16) + encCtxSeq
-      case EmptyAAD() =>
-        UInt16ToSeq(0)
-    }
+    reveal ValidAAD();
+    match aad
+    case AAD(kvPairs) =>
+      var n := |kvPairs|;
+      UInt16ToSeq(AADLength(aad) as uint16) +
+      UInt16ToSeq(n as uint16) +
+      SerializeKVPairs(kvPairs, 0, n)
+    case EmptyAAD() =>
+      UInt16ToSeq(0)
   }
+
+  function SerializeKVPairs(kvPairs: EncCtx, lo: nat, hi: nat): seq<uint8>
+    requires forall i :: 0 <= i < |kvPairs| ==> ValidKVPair(kvPairs[i])
+    requires lo <= hi <= |kvPairs|
+  {
+    if lo == hi then [] else SerializeKVPairs(kvPairs, lo, hi - 1) + SerializeKVPair(kvPairs[hi - 1])
+  }
+
+  function SerializeKVPair(kvPair: (seq<uint8>, seq<uint8>)): seq<uint8>
+    requires ValidKVPair(kvPair)
+  {
+    UInt16ToSeq(|kvPair.0| as uint16) + kvPair.0 +
+    UInt16ToSeq(|kvPair.1| as uint16) + kvPair.1
+  }
+
+  // Function AADLength is defined without referring to SerializeAAD (because then
+  // these two would be mutually recursive with ValidAAD). The following lemma proves
+  // that the two definitions correspond.
+  lemma ADDLengthCorrect(aad: T_AAD)
+    requires ValidAAD(aad)
+    ensures |SerializeAAD(aad)| == 2 + AADLength(aad)
+  {
+    reveal ValidAAD();
+    match aad
+    case AAD(kvPairs) =>
+      KVPairsLengthCorrect(kvPairs, 0, |kvPairs|);
+      /**** Here's a more detailed proof:
+      var n := |kvPairs|;
+      var s := SerializeKVPairs(kvPairs, 0, n);
+      calc {
+        |SerializeAAD(aad)|;
+      ==  // def. SerializeAAD
+        |UInt16ToSeq(AADLength(aad) as uint16) + UInt16ToSeq(n as uint16) + s|;
+      ==  // UInt16ToSeq yields length-2 sequence
+        2 + 2 + |s|;
+      ==  { KVPairsLengthCorrect(kvPairs, 0, n); }
+        2 + 2 + KVPairsLength(kvPairs, 0, n);
+      }
+      ****/
+    case EmptyAAD() =>
+  }
+
+  lemma KVPairsLengthCorrect(kvPairs: EncCtx, lo: nat, hi: nat)
+    requires forall i :: 0 <= i < |kvPairs| ==> ValidKVPair(kvPairs[i])
+    requires lo <= hi <= |kvPairs|
+    ensures |SerializeKVPairs(kvPairs, lo, hi)| == KVPairsLength(kvPairs, lo, hi)
+  {
+    /**** Here's a more detailed proof:
+    if lo < hi {
+      var kvPair := kvPairs[hi - 1];
+      calc {
+        |SerializeKVPairs(kvPairs, lo, hi)|;
+      ==  // def. SerializeKVPairs
+        |SerializeKVPairs(kvPairs, lo, hi - 1) + SerializeKVPair(kvPair)|;
+      ==
+        |SerializeKVPairs(kvPairs, lo, hi - 1)| + |SerializeKVPair(kvPair)|;
+      ==  { KVPairsLengthCorrect(kvPairs, lo, hi - 1); }
+        KVPairsLength(kvPairs, lo, hi - 1) + |SerializeKVPair(kvPair)|;
+      ==  // def. SerializeKVPair
+        KVPairsLength(kvPairs, lo, hi - 1) +
+        |UInt16ToSeq(|kvPair.0| as uint16) + kvPair.0 + UInt16ToSeq(|kvPair.1| as uint16) + kvPair.1|;
+      ==
+        KVPairsLength(kvPairs, lo, hi - 1) + 2 + |kvPair.0| + 2 + |kvPair.1|;
+      ==  // def. KVPairsLength
+        KVPairsLength(kvPairs, lo, hi);
+      }
+    }
+    ****/
+  }
+
+  // ----- Implementation -----
 
   method SerializeAADImpl(os: Streams.StringWriter, aad: T_AAD) returns (ret: Result<nat>)
     requires os.Valid() && ValidAAD(aad)
@@ -64,118 +113,88 @@ module MessageHeader.SerializeAAD {
         && os.data == old(os.data) + serAAD
       case Failure(e) => true
   {
+    reveal ValidAAD();
+
     var totalWritten := 0;
     ghost var initLen := |os.data|;
-    ghost var written: seq<nat> := [initLen];
-    ghost var i := 0;
 
     match aad {
       case AAD(kvPairs) =>
-        var len: nat;
-        {
-          // Key Value Pairs Length (number of bytes of total AAD)
-          var length: uint16;
-          assert InBoundsKVPairs(kvPairs) ==> |kvPairs| < UINT16_LIMIT;
-          // TODO: We need to compute length here after removing length field from AAD datatype
-          Assume(forall i :: 0 <= i < |kvPairs| ==> |kvPairs[i].0| < UINT16_LIMIT && |kvPairs[i].1| < UINT16_LIMIT);
-          Assume(length == |EncCtxToSeq(kvPairs)| as uint16);
-          var bytes := UInt16ToArray(length);
-          len :- os.WriteSimple(bytes);
-          totalWritten := totalWritten + len;
-          i := i + 1;
-          written := written + [initLen + totalWritten];
-          assert written[i] - written[i-1] == bytes.Length;
-          assert written[i-1] <= written[i] <= |os.data| ==> os.data[written[i-1]..written[i]] == bytes[..];
-          Assume(ValidAAD(aad));  // TODO
-          assert totalWritten <= |SerializeAAD(aad)|;
-        }
+        // Key Value Pairs Length (number of bytes of total AAD)
+        var length :- ComputeAADLength(aad);
+        var bytes := UInt16ToSeq(length);
+        var len :- os.WriteSimpleSeq(bytes);
+        totalWritten := totalWritten + len;
+        assert totalWritten == 2;
 
-        Assume(0 < |kvPairs|);
-        assert 0 < |kvPairs|;
-        {
-          assert InBoundsKVPairs(kvPairs) ==> |kvPairs| < UINT16_LIMIT;
-          // Key Value Pair Count (number of key value pairs)
-          Assume(|kvPairs| < UINT16_LIMIT);
-          var bytes := UInt16ToArray(|kvPairs| as uint16);
-          len :- os.WriteSimple(bytes);
-          totalWritten := totalWritten + len;
-          i := i + 1;
-          written := written + [initLen + totalWritten];
-          assert written[i] - written[i-1] == bytes.Length;
-          assert written[i-1] <= written[i] <= |os.data| ==> os.data[written[i-1]..written[i]] == bytes[..];
-          Assume(ValidAAD(aad));  // TODO
-          assert totalWritten <= |SerializeAAD(aad)|;
-        }
-
-        Assume(false); // TODO: verification times out after this point. I believe that we just do too many heap updates.
+        bytes := UInt16ToSeq(|kvPairs| as uint16);
+        len :- os.WriteSimpleSeq(bytes);
+        totalWritten := totalWritten + len;
+        assert totalWritten == 4;
 
         var j := 0;
+        ghost var n := |kvPairs|;
         while j < |kvPairs|
-          invariant j <= |kvPairs|
-          invariant unchanged(os`Repr)
-          invariant InBoundsKVPairsUpTo(kvPairs, j)
-          invariant ValidAAD(aad)
-          invariant totalWritten <= |SerializeAAD(aad)|
-          invariant initLen+totalWritten <= |os.data|
-          invariant SerializeAAD(aad)[written[i-1]-initLen..written[i]-initLen] == os.data[written[i-1]..written[i]];
-          //invariant SerializeAAD(aad)[..totalWritten] == os.data[initLen..written[i]];
+          invariant j <= n == |kvPairs|
+          invariant os.data ==
+            old(os.data) +
+            UInt16ToSeq(length) +
+            UInt16ToSeq(n as uint16) +
+            SerializeKVPairs(kvPairs, 0, j)
+          invariant totalWritten == 4 + |SerializeKVPairs(kvPairs, 0, j)|
         {
-          {
-            assert InBoundsKVPairsUpTo(kvPairs, j) ==> |kvPairs[j].0| < UINT16_LIMIT;
-            var bytes := UInt16ToArray(|kvPairs[j].0| as uint16);
-            len :- os.WriteSimple(bytes);
-            totalWritten := totalWritten + len;
-            i := i + 1;
-            written := written + [initLen + totalWritten];
-            assert written[i] - written[i-1] == bytes.Length;
-            assert written[i-1] <= written[i] <= |os.data| ==> os.data[written[i-1]..written[i]] == bytes[..];
-          }
+          bytes := UInt16ToSeq(|kvPairs[j].0| as uint16);
+          len :- os.WriteSimpleSeq(bytes);
+          totalWritten := totalWritten + len;
 
-          {
-            var bytes := kvPairs[j].0;
-            len :- os.WriteSimpleSeq(bytes);
-            totalWritten := totalWritten + len;
-            i := i + 1;
-            written := written + [initLen + totalWritten];
-            assert written[i] - written[i-1] == |bytes|;
-            assert written[i-1] <= written[i] <= |os.data| ==> os.data[written[i-1]..written[i]] == bytes[..];
-          }
+          len :- os.WriteSimpleSeq(kvPairs[j].0);
+          totalWritten := totalWritten + len;
 
-          {
-            assert InBoundsKVPairsUpTo(kvPairs, j) ==> |kvPairs[j].1| < UINT16_LIMIT;
-            var bytes := UInt16ToSeq(|kvPairs[j].1| as uint16);
-            len :- os.WriteSimpleSeq(bytes);
-            totalWritten := totalWritten + len;
-            i := i + 1;
-            written := written + [initLen + totalWritten];
-            assert written[i] - written[i-1] == |bytes|;
-            assert written[i-1] <= written[i] <= |os.data| ==> os.data[written[i-1]..written[i]] == bytes[..];
-          }
+          bytes := UInt16ToSeq(|kvPairs[j].1| as uint16);
+          len :- os.WriteSimpleSeq(bytes);
+          totalWritten := totalWritten + len;
 
-          {
-            var bytes := kvPairs[j].1;
-            len :- os.WriteSimpleSeq(bytes);
-            totalWritten := totalWritten + len;
-            i := i + 1;
-            written := written + [initLen + totalWritten];
-            assert written[i] - written[i-1] == |bytes|;
-            assert written[i-1] <= written[i] <= |os.data| ==> os.data[written[i-1]..written[i]] == bytes[..];
-          }
+          len :- os.WriteSimpleSeq(kvPairs[j].1);
+          totalWritten := totalWritten + len;
 
           j := j + 1;
         }
-        return Success(len);
+        
+        return Success(totalWritten);
 
       case EmptyAAD() =>
         var bytes := UInt16ToArray(0);
         var len :- os.WriteSimple(bytes);
-        totalWritten := totalWritten + len;
-        i := i + 1;
-        written := written + [initLen + totalWritten];
-        assert written[i] - written[i-1] == 2;
-        assert written[i-1] <= written[i] <= |os.data| ==> os.data[written[i-1]..written[i]] == bytes[..];
-        Assume(ValidAAD(aad));
+        assert len == 2;
         return Success(len);
     }
+  }
+
+  method ComputeAADLength(aad: T_AAD) returns (res: Result<uint16>)
+    requires aad.AAD? ==> |aad.kvPairs| < UINT16_LIMIT
+    requires aad.AAD? ==> forall i :: 0 <= i < |aad.kvPairs| ==> ValidKVPair(aad.kvPairs[i])
+    ensures match res
+      case Success(len) => len as int == AADLength(aad)
+      case Failure(_) => UINT16_LIMIT <= AADLength(aad)
+  {
+    match aad
+    case AAD(kvPairs) =>
+      var len: int32, limit: int32 := 2, UINT16_LIMIT as int32;
+      var i: int32, n: int32 := 0, |aad.kvPairs| as int32;
+      while i < n
+        invariant i <= n == |aad.kvPairs| as int32
+        invariant 2 + KVPairsLength(kvPairs, 0, i as int) == len as int < UINT16_LIMIT == limit as int
+      {
+        var kvPair := kvPairs[i];
+        len := len + 4 + |kvPair.0| as int32 + |kvPair.1| as int32;
+        KVPairsLengthSplit(kvPairs, 0, i as int + 1, n as int);
+        if limit <= len {
+          return Failure("The number of bytes in encryption context exceeds the allowed maximum");
+        }
+        i := i + 1;
+      }
+      return Success(len as uint16);
+    case EmptyAAD() =>
+      return Success(0);
   }
 }
