src/SDK/MessageHeader/Serialize.dfy
@@ -1,7 +1,3 @@
-// This file verified before removing length/count from the AAD/EDK datatypes
-// with Dafny flag -arith:5 and when commenting out the HeapSucc transitivity axiom in the DafnyPrelude.bpl.
-// Turned the failing assertion into an assume for now.
-
 include "Definitions.dfy"
 include "SerializeAAD.dfy"
 include "SerializeEDK.dfy"
@@ -20,9 +16,6 @@ module MessageHeader.Serialize {
   import opened StandardLibrary
   import opened UInt = StandardLibrary.UInt
 
-  lemma {:axiom} Assume(b: bool)
-    ensures b
-
   function {:opaque} Serialize(hb: HeaderBody): seq<uint8>
     requires ValidHeaderBody(hb)
   {
@@ -32,7 +25,7 @@ module MessageHeader.Serialize {
     UInt16ToSeq(hb.algorithmSuiteID as uint16) +
     hb.messageID +
     SerializeAAD.SerializeAAD(hb.aad) +
-    SerializeEDK.SerializeEDK(hb.encryptedDataKeys) +
+    SerializeEDK.SerializeEDKs(hb.encryptedDataKeys) +
     (match hb.contentType case NonFramed => [0x01] case Framed => [0x02]) +
     hb.reserved +
     [hb.ivLength] +
@@ -56,10 +49,6 @@ module MessageHeader.Serialize {
       case Failure(e) => true
   {
     var totalWritten := 0;
-    ghost var initLen := |os.data|;
-    reveal ValidHeaderBody();
-    reveal ValidAAD();
-    reveal ValidEncryptedDataKeys();
 
     var len :- os.WriteSingleByteSimple(hb.version as uint8);
     totalWritten := totalWritten + len;
@@ -74,10 +63,11 @@ module MessageHeader.Serialize {
     len :- os.WriteSimpleSeq(hb.messageID);
     totalWritten := totalWritten + len;
 
+    reveal ValidHeaderBody();
     len :- SerializeAAD.SerializeAADImpl(os, hb.aad);
     totalWritten := totalWritten + len;
 
-    len :- SerializeEDK.SerializeEDKImpl(os, hb.encryptedDataKeys);
+    len :- SerializeEDK.SerializeEDKsImpl(os, hb.encryptedDataKeys);
     totalWritten := totalWritten + len;
 
     var contentType: uint8;
@@ -98,17 +88,7 @@ module MessageHeader.Serialize {
     len :- os.WriteSimple(bytes);
     totalWritten := totalWritten + len;
 
-    Assume(false);
-    //reveal ReprEncryptedDataKeys();
-    assert ValidHeaderBody(hb);
     reveal Serialize();
-    ghost var serHb := Serialize(hb);
-    assert totalWritten == |serHb|;
-    assert initLen+totalWritten == |os.data|;
-
-    // Turned this assertion into an assume. This assertion worked before removing the length/count from AAD/EDK datatypes
-    Assume(serHb[..totalWritten] == os.data[initLen..initLen+totalWritten]);
-
     return Success(totalWritten);
   }
 }
